clean up mono proof (separate unrolling)

src/parlang_nonmono.lean
@@ -2,6 +2,7 @@ import parlang
 
 namespace parlang_nonmono
 variables {n : ℕ} {σ : Type} {ι : Type} {τ : ι → Type} [decidable_eq ι]
+notation `v[` v:(foldr `, ` (h t, vector.cons h t) vector.nil `]`) := v
 
 open parlang
 open parlang.kernel
@@ -24,42 +25,19 @@ inductive exec_state {n : ℕ} : kernel σ τ → vector bool n → state n σ �
   exec_state k₁ (deactivate_threads (bnot ∘ f) ac s) s t →
   exec_state k₂ (deactivate_threads f ac s) t u →
   exec_state (ite f k₁ k₂) ac s u
-  -- in the then-branch we deactive those threads where the condition is false and vice versa
 | loop_stop (s : state n σ τ) (ac : vector bool n) (f : σ → bool) (k : kernel σ τ) :
   no_thread_active (deactivate_threads (bnot ∘ f) ac s) →
   exec_state (loop f k) ac s s
 | loop_step (s t u : state n σ τ) (ac : vector bool n) (f : σ → bool) (k : kernel σ τ) :
   any_thread_active (deactivate_threads (bnot ∘ f) ac s) →
   exec_state k (deactivate_threads (bnot ∘ f) ac s) s t →
+-- the only difference to to parlang is the line below; here we don't deactivate threads
   exec_state (loop f k) ac t u →
   exec_state (loop f k) ac s u
 
-
-def contains_sync : kernel σ τ → Prop
-| sync := true
-| (seq a b) := (contains_sync a) ∨ (contains_sync b)
-| (ite _ a b) := (contains_sync a) ∨ (contains_sync b)
-| (loop _ a) := (contains_sync a)
-| _ := false
-
-instance decidable (k : kernel σ τ) : decidable (contains_sync k) := sorry
-
-variables {s t u : state n σ τ} {ac : vector bool n} {f f' : σ → bool} {semantics : kernel σ τ → vector bool n → state n σ τ → state n σ τ → Prop}
-
-class has_unique (semantics : kernel σ τ → vector bool n → state n σ τ → state n σ τ → Prop) := 
-(unique : ∀ {k : kernel σ τ} {ac : vector bool n} {s t t' : state n σ τ}, semantics k ac s t → semantics k ac s t' → t = t')
-
-variables [has_unique semantics]
-
-instance unique2 : has_unique $ @parlang.exec_state σ ι τ _ n := ⟨begin
-    intros _ _ _ _ _ a b,
-    apply parlang.exec_state_unique b a,
-end⟩
-
-instance unique1 : has_unique $ @exec_state σ ι τ _ n := sorry
+variables {s t u : state n σ τ} {ac : vector bool n} {f f' : σ → bool} 
 
 def ac_ge (ac' : vector bool n) (ac : vector bool n) : Prop := ∀ (t : fin n), ¬ (ac.nth t) → ¬ (ac'.nth t)
-
 instance : has_le (vector bool n) := ⟨ac_ge⟩
 
 lemma exec_state_inactive_threads_untouched {s u : state n σ τ} {ac : vector bool n} {k} : exec_state k ac s u → ∀ i, ¬ ac.nth i → s.threads.nth i = u.threads.nth i := begin
@@ -101,64 +79,6 @@ deactivate_threads (bnot ∘ f) ac s ≥ deactivate_threads (bnot ∘ f) ac t :=
     admit,
 end
 
--- probably has to be an inducive type
--- def ac_after_n_iteration (k : kernel σ τ) (f : σ → bool) : ℕ → state n σ τ → vector bool n → vector bool n
--- | 0 s ac := ac
--- | (n + 1) s ac := if (∃ t, exec_state k ac s t) then ac_after_n_iteration n t (deactivate_threads (bnot ∘ f) ac s) else ac -- all false
-
--- this is similar to the semantic itself except we are not interested in states but the resulting active maps
--- it is reversed, maybe we should build it the other way around
-inductive ac_after_n_iteration (semantics : kernel σ τ → vector bool n → state n σ τ → state n σ τ → Prop) (k : kernel σ τ) (f : σ → bool) : state n σ τ → vector bool n → vector bool n → ℕ → Prop
-| base (ac : vector bool n) (s : state n σ τ) : ac_after_n_iteration s ac ac 0
-| step {ac : vector bool n} (s t : state n σ τ) {i : ℕ} {ac' : vector bool n} : ac_after_n_iteration t (deactivate_threads (bnot ∘ f) ac s) ac' i → semantics k (deactivate_threads (bnot ∘ f) ac s) s t → ac_after_n_iteration s ac ac' (i + 1)
---| step (ac : vector bool n) (s t : state n σ τ) (i : ℕ) (ac' : vector bool n) : ac_after_n_iteration s ac ac' i → exec_state k ac' s t → ac_after_n_iteration s ac (deactivate_threads (bnot ∘ f) ac t) (i + 1)
-
--- this semantic would require that in and out ac are always the same
-inductive ac_after_n_iteration_nonmono (semantics : kernel σ τ → vector bool n → state n σ τ → state n σ τ → Prop) (k : kernel σ τ) (f : σ → bool) : state n σ τ → vector bool n → vector bool n → ℕ → Prop
-| base (ac : vector bool n) (s : state n σ τ) : ac_after_n_iteration_nonmono s ac ac 0
-| step {ac : vector bool n} (s t : state n σ τ) {i : ℕ} {ac' : vector bool n} : ac_after_n_iteration_nonmono t ac ac' i → semantics k (deactivate_threads (bnot ∘ f) ac s) s t → ac_after_n_iteration_nonmono s ac ac' (i + 1)
-
-example {k f} {ac' : vector bool n} {i} : ac_after_n_iteration semantics k f s ac ac' i ↔ ac_after_n_iteration_nonmono semantics k f s ac ac' i := begin
-    split, {
-        revert ac ac' s,
-        induction i,
-        case nat.zero {
-            intros ac ac' s h,
-            cases h,
-            apply ac_after_n_iteration_nonmono.base,
-        },
-        case nat.succ {
-            intros ac ac' s h,
-            cases h,
-            rename h_t t,
-            apply ac_after_n_iteration_nonmono.step,
-            swap,
-            exact h_a_1,
-            apply i_ih,
-            clear i_ih,
-            cases i_n,
-            case nat.zero {
-
-            }
-            
-        }
-    }
-end
-
-notation `v[` v:(foldr `, ` (h t, vector.cons h t) vector.nil `]`) := v
-
-example : ac_after_n_iteration exec_state (compute (λ (m : bool), ff)) id (@parlang.init_state bool string (λs, ℕ) _ (λ_, tt) (λ_,1) (λs:string, 0)) v[tt] v[tt] 1 := begin
-    apply ac_after_n_iteration.step _ (@parlang.init_state bool string (λs, ℕ) _ (λ_, ff) (λ_,1) (λs:string, 0)),
-    swap,
-    sorry,
-    apply ac_after_n_iteration.base,
-end
-
-lemma ac_after_n_iteration_unique {k : kernel σ τ} {f : σ → bool} {ac' ac'' : vector bool n} {i} : 
-ac_after_n_iteration semantics k f s ac ac' i → ac_after_n_iteration semantics k f s ac ac'' i → ac' = ac'' := begin
-    admit,
-end
-
 lemma ac_sub_deac {f : σ → bool} : ac ≥ (deactivate_threads (bnot ∘ f) ac s) := begin
     intros t h₁ h₂,
     apply h₁,
@@ -188,129 +108,6 @@ end
 lemma ac_deac_ge (h : deactivate_threads f ac s ≥ deactivate_threads f' ac t) : deactivate_threads f' (deactivate_threads f ac s) t = deactivate_threads f' ac t := begin
     admit,
 end
-
-lemma ac_ge_single {k : kernel σ τ} {f : σ → bool} {ac' : vector bool n} {i : ℕ} : ac_after_n_iteration semantics k f s ac ac' i → ac ≥ ac' := begin
-    intros h,
-    induction i generalizing s ac ac',
-    case nat.zero {
-        cases h,
-        intros t hna,
-        assumption,
-    },
-    case nat.succ {
-        cases h,
-        specialize i_ih h_a,
-        have : ac ≥ (deactivate_threads (bnot ∘ f) ac s) := by apply ac_sub_deac,
-        sorry, -- proof by transitivity
-    }
-end
-
-lemma ac_ge_two {k : kernel σ τ} {f : σ → bool} {i i' : ℕ} {ac' ac'' : vector bool n} : 
-ac_after_n_iteration semantics k f s ac ac' i → ac_after_n_iteration semantics k f s ac ac'' (i + i') → ac' ≥ ac'' := begin
-    intros h₁ h₂,
-    induction i generalizing s ac,
-    case nat.zero {
-        cases h₁,
-        apply ac_ge_single h₂,
-    },
-    case nat.succ {
-        cases h₁,
-        have : nat.succ i_n + i' = nat.succ (i_n + i') := by rw nat.succ_add,
-        rw this at h₂,
-        cases h₂,
-        have : h₁_t = h₂_t := has_unique.unique _ _ _ h₁_a_1 h₂_a_1,
-        subst this,
-        apply i_ih h₁_a h₂_a,
-    }
-end
-
-#print parlang_nonmono.exec_state.rec_on
-
-lemma loop_ac {k : kernel σ τ}  (h : exec_state (loop f k) ac s t) : ∃ i ac', ac_after_n_iteration exec_state k f s ac ac' i ∧ no_thread_active (deactivate_threads (bnot ∘ f) ac' t)
-:= h.rec_on 
-    (λ f s ac, _)
-    _
-    _
-    _
-    _
-    _
-    _
-    _
-    (λ s t u ac f k h₁ h₂ h₃ ih₁ (ih₂ : ∃ (i : ℕ) (ac' : vector bool n), ac_after_n_iteration exec_state k f s ac ac' i ∧ ↥(no_thread_active (deactivate_threads (bnot ∘ f) ac' t))), (show ∃ i ac', ac_after_n_iteration exec_state k f s ac ac' i ∧ no_thread_active (deactivate_threads (bnot ∘ f) ac' t), by begin 
-
-    end))
-
-def monotone_loop (semantics : kernel σ τ → vector bool n → state n σ τ → state n σ τ → Prop) (f k) (s : state n σ τ) (ac : vector bool n) : Prop := 
-∀ (i i' : ℕ) (ac' ac'' : vector bool n), ac_after_n_iteration semantics k f s ac ac' i → ac_after_n_iteration semantics k f s ac ac'' (i + i') → ac' ≥ ac''
-
-lemma par_loop_ac' {k : kernel σ τ} : parlang.exec_state (loop f k) ac s t → ∃ i ac', ac_after_n_iteration parlang.exec_state k f s ac ac' i ∧ no_thread_active (deactivate_threads (bnot ∘ f) ac' t) := begin
-    generalize eq_l : (loop f k) = l,
-    intro h,
-    induction h;
-        cases eq_l,
-    {
-        use 0,
-        use h_ac,
-        split,
-        apply ac_after_n_iteration.base,
-        assumption,
-    }, {
-        clear h_ih_a,
-        specialize h_ih_a_1 rfl,
-        cases h_ih_a_1 with i ih,
-        cases ih with ac' ih,
-        cases ih with ha hb,
-        use i + 1,
-        use ac',
-        split,
-        swap,
-        assumption,
-        apply ac_after_n_iteration.step,
-        repeat { assumption },
-    }
-end
-
-lemma loop_ac' {k : kernel σ τ} : exec_state (loop f k) ac s t ↔ ∃ i ac', ac_after_n_iteration exec_state k f s ac ac' i ∧ no_thread_active (deactivate_threads (bnot ∘ f) ac' t) := begin
-    split,
-    {
-        generalize eq_l : (loop f k) = l,
-        intro h,
-        induction h generalizing;
-            cases eq_l,
-        {
-            use 0,
-            use h_ac,
-            split,
-            apply ac_after_n_iteration.base,
-            assumption,
-        }, {
-            clear h_ih_a,
-            specialize h_ih_a_1 rfl,
-            cases h_ih_a_1 with i ih,
-            cases ih with ac' ih,
-            cases ih with ha hb,
-            use i + 1,
-            use ac',
-            split,
-            swap,
-            assumption,
-            {
-                apply ac_after_n_iteration.step,
-                swap,
-                exact h_a_1,
-                induction ha,
-                case parlang_nonmono.ac_after_n_iteration.base {
-                    have : monotone_loop exec_state f k h_s ha_ac := by apply ac_ge_two,
-                    have : monotone_loop exec_state f k h_s ha_ac := by apply ac_ge_two,
-                }
-            }
-        }
-    }
-end
-
-#print loop_ac'
-
-#print deactivate_threads._match_1
 
 lemma vv {k} (ha : any_thread_active (deactivate_threads (bnot ∘ f) ac s)) (hi : exec_state k (deactivate_threads (bnot ∘ f) ac s) s t) (h : exec_state (loop f k) (deactivate_threads (bnot ∘ f) ac s) t u) :
 exec_state (loop f k) ac s u := begin
