src/ac_loop.lean
@@ -1,0 +1,145 @@
+import parlang
+import parlang_nonmono
+
+namespace parlang
+namespace ac_loop
+
+open parlang
+open parlang.kernel
+open parlang_nonmono
+
+variables {n : ℕ} {σ : Type} {ι : Type} {τ : ι → Type} {s t u : state n σ τ} {ac : vector bool n} {f f' : σ → bool}  [decidable_eq ι] {semantics : kernel σ τ → vector bool n → state n σ τ → state n σ τ → Prop}
+
+class has_unique (semantics : kernel σ τ → vector bool n → state n σ τ → state n σ τ → Prop) := 
+(unique : ∀ {k : kernel σ τ} {ac : vector bool n} {s t t' : state n σ τ}, semantics k ac s t → semantics k ac s t' → t = t')
+
+variables [has_unique semantics]
+
+instance unique2 : has_unique $ @parlang.exec_state σ ι τ _ n := ⟨begin
+    intros _ _ _ _ _ a b,
+    apply parlang.exec_state_unique b a,
+end⟩
+
+instance unique1 : has_unique $ @exec_state σ ι τ _ n := sorry
+
+notation `v[` v:(foldr `, ` (h t, vector.cons h t) vector.nil `]`) := v
+
+-- this is similar to the semantic itself except we are not interested in states but the resulting active maps
+inductive ac_after_n_iteration (semantics : kernel σ τ → vector bool n → state n σ τ → state n σ τ → Prop) (k : kernel σ τ) (f : σ → bool) : state n σ τ → vector bool n → vector bool n → ℕ → Prop
+| base (ac : vector bool n) (s : state n σ τ) : ac_after_n_iteration s ac ac 0
+| step {ac : vector bool n} (s t : state n σ τ) {i : ℕ} {ac' : vector bool n} : ac_after_n_iteration t (deactivate_threads (bnot ∘ f) ac s) ac' i → semantics k (deactivate_threads (bnot ∘ f) ac s) s t → ac_after_n_iteration s ac ac' (i + 1)
+
+example : ac_after_n_iteration exec_state (compute (λ (m : bool), ff)) id (@parlang.init_state bool string (λs, ℕ) _ (λ_, tt) (λ_,1) (λs:string, 0)) v[tt] v[tt] 1 := begin
+    apply ac_after_n_iteration.step _ (@parlang.init_state bool string (λs, ℕ) _ (λ_, ff) (λ_,1) (λs:string, 0)),
+    swap,
+    sorry,
+    sorry,
+end
+
+lemma ac_after_n_iteration_unique {k : kernel σ τ} {f : σ → bool} {ac' ac'' : vector bool n} {i} : 
+ac_after_n_iteration semantics k f s ac ac' i → ac_after_n_iteration semantics k f s ac ac'' i → ac' = ac'' := begin
+    admit,
+end
+
+lemma ac_ge_single {k : kernel σ τ} {f : σ → bool} {ac' : vector bool n} {i : ℕ} : ac_after_n_iteration semantics k f s ac ac' i → ac ≥ ac' := begin
+    intros h,
+    induction i generalizing s ac ac',
+    case nat.zero {
+        cases h,
+        intros t hna,
+        assumption,
+    },
+    case nat.succ {
+        cases h,
+        specialize i_ih h_a,
+        have : ac ≥ (deactivate_threads (bnot ∘ f) ac s) := by apply ac_sub_deac,
+        sorry, -- proof by transitivity
+    }
+end
+
+lemma ac_ge_two {k : kernel σ τ} {f : σ → bool} {i i' : ℕ} {ac' ac'' : vector bool n} : 
+ac_after_n_iteration semantics k f s ac ac' i → ac_after_n_iteration semantics k f s ac ac'' (i + i') → ac' ≥ ac'' := begin
+    intros h₁ h₂,
+    induction i generalizing s ac,
+    case nat.zero {
+        cases h₁,
+        apply ac_ge_single h₂,
+    },
+    case nat.succ {
+        cases h₁,
+        have : nat.succ i_n + i' = nat.succ (i_n + i') := by rw nat.succ_add,
+        rw this at h₂,
+        cases h₂,
+        have : h₁_t = h₂_t := has_unique.unique _ _ _ h₁_a_1 h₂_a_1,
+        subst this,
+        apply i_ih h₁_a h₂_a,
+    }
+end
+
+def monotone_loop (semantics : kernel σ τ → vector bool n → state n σ τ → state n σ τ → Prop) (f k) (s : state n σ τ) (ac : vector bool n) : Prop := 
+∀ (i i' : ℕ) (ac' ac'' : vector bool n), ac_after_n_iteration semantics k f s ac ac' i → ac_after_n_iteration semantics k f s ac ac'' (i + i') → ac' ≥ ac''
+
+lemma par_loop_ac' {k : kernel σ τ} : parlang.exec_state (loop f k) ac s t → ∃ i ac', ac_after_n_iteration parlang.exec_state k f s ac ac' i ∧ no_thread_active (deactivate_threads (bnot ∘ f) ac' t) := begin
+    generalize eq_l : (loop f k) = l,
+    intro h,
+    induction h;
+        cases eq_l,
+    {
+        use 0,
+        use h_ac,
+        split,
+        apply ac_after_n_iteration.base,
+        assumption,
+    }, {
+        clear h_ih_a,
+        specialize h_ih_a_1 rfl,
+        cases h_ih_a_1 with i ih,
+        cases ih with ac' ih,
+        cases ih with ha hb,
+        use i + 1,
+        use ac',
+        split,
+        swap,
+        assumption,
+        apply ac_after_n_iteration.step,
+        repeat { assumption },
+    }
+end
+
+lemma loop_ac' {k : kernel σ τ} : exec_state (loop f k) ac s t → ∃ i ac', ac_after_n_iteration exec_state k f s ac ac' i ∧ no_thread_active (deactivate_threads (bnot ∘ f) ac' t) := begin
+    generalize eq_l : (loop f k) = l,
+    intro h,
+    induction h generalizing;
+        cases eq_l,
+    {
+        use 0,
+        use h_ac,
+        split,
+        apply ac_after_n_iteration.base,
+        assumption,
+    }, {
+        clear h_ih_a,
+        specialize h_ih_a_1 rfl,
+        cases h_ih_a_1 with i ih,
+        cases ih with ac' ih,
+        cases ih with ha hb,
+        use i + 1,
+        use ac',
+        split,
+        swap,
+        assumption,
+        {
+            apply ac_after_n_iteration.step,
+            swap,
+            exact h_a_1,
+            induction ha,
+            case ac_after_n_iteration.base {
+                have : monotone_loop exec_state f k h_s ha_ac := by apply ac_ge_two,
+                have : monotone_loop exec_state f k h_s ha_ac := by apply ac_ge_two,
+            }
+        }
+    }
+end
+
+end ac_loop
+end parlang
